theories/soundness/setc.v
@@ -15,49 +15,56 @@ From shack Require Import heap modality interp typing.
 From shack.soundness Require Import expr defs.
 
 Section proofs.
-  (* assume a given set of class definitions *)
-  Context `{PDC: ProgDefContext}.
-  (* assume some SDT constraints and their properties *)
-  Context `{SDTCS: SDTClassSpec}.
+  (* assume a given set of class definitions and their SDT annotations. *)
+  Context `{SDTCVS: SDTClassVarianceSpec}.
 
   (* Iris semantic context *)
   Context `{!sem_heapGS Θ}.
 
-  Lemma set_priv_soundness C Δ kd rigid Γ fld rhs fty t σ:
+  Lemma set_priv_soundness C Δ kd cdef rigid Γ fld rhs fty:
     wf_cdefs pdefs →
     wf_lty Γ →
     Forall wf_constraint Δ →
-    type_of_this Γ = (t, σ) →
-    has_field fld t Private fty C →
-    expr_has_ty Δ Γ rigid kd rhs (subst_ty σ fty) →
+    pdefs !! C = Some cdef →
+    cdef.(classfields) !! fld = Some (Private, fty) →
+    expr_has_ty Δ Γ rigid kd rhs fty →
+    ∀ t tdef Σt σ,
+    pdefs !! t = Some tdef →
+    length Σt = length tdef.(generics) →
+    inherits_using t C σ →
     ∀ Σ st st' n,
     length Σ = rigid →
     cmd_eval C st (SetC ThisE fld rhs) st' n →
+    let Σthis := interp_exact_tag interp_type t Σt in
+    ⌜interp_list interp_nothing Σt σ ≡ Σ⌝ -∗
+    □ interp_env_as_mixed Σt -∗
     □ interp_env_as_mixed Σ -∗
-    □ Σinterp Σ Δ -∗
-    heap_models st.2 ∗ interp_local_tys Σ Γ st.1 -∗
-    |=▷^n heap_models st'.2 ∗ interp_local_tys Σ Γ st'.1.
+    □ Σinterp Σthis Σ Δ -∗
+    heap_models st.2 ∗ interp_local_tys Σthis Σ Γ st.1 -∗
+    |=▷^n heap_models st'.2 ∗ interp_local_tys Σthis Σ Γ st'.1.
   Proof.
-    move => wfpdefs wflty ? hthis hf hrhs Σ st st' n hrigid hc.
+    move => wfpdefs.
+    destruct wfpdefs.
+    move => wflty ? hcdef hf hrhs.
+    move => t tdef Σt σ htdef hlenΣt hin_t_C.
+    move => Σ st st' n hrigid hc Σthis.
     elim/cmd_eval_setI : hc => {n}.
-    move => Ω h l v t0 vs vs' heval heval_rhs hheap -> hvis.
-    iIntros "#hΣ #hΣΔ".
+    move => Ω h vis fty0 orig l v t0 vs vs' heval heval_rhs hheap ->.
+    move => hf0 hvis /=.
+    iIntros "%hΣeq #hΣt #hΣ #hΣΔ".
     iIntros "[Hh #Hle]" => /=.
     iSplitL; last done.
-    destruct Γ as [[tthis σthis]  Γ].
     destruct Ω as [vthis Ω].
-    injection hthis; intros; subst; clear hthis.
-    assert (ht: wf_ty (ClassT true t σ)).
-    { eapply wf_ty_exact; by apply wflty. }
-    iApply (heap_models_update Δ _ _ _ _ _ false t σ) => //=; try (by apply wfpdefs).
-    - iDestruct "Hle" as "[Hthis Hle]".
-      rewrite /= /interp_this_type interp_this_unseal /interp_this_def /=.
-      iDestruct "Hthis" as (l' t1 def1 σ0 σt fields ifields) "(%H & #hmixed & #? & #hinst & #hdyn & #Hl)".
-      destruct H as ([= <-] & hdef1 & ? & hin & hfields & hidom).
-      iExists l, t1, def1, σ0, σt, fields, ifields.
-      repeat iSplit => //.
-      by case: heval => ->.
-    - iApply expr_soundness => //; by apply wfpdefs.
+    case: heval heval_rhs => -> heval_rhs {vthis}.
+    iAssert (□ interp_as_mixed Σthis)%I as "#hΣthis".
+    { iModIntro; iIntros (w) "hw".
+      iLeft; iRight; iRight.
+      iExists t, Σt, tdef; iSplit; first done.
+      by iApply (exact_subtype_is_inclusion_aux with "hΣt hw").
+    }
+    iApply (heap_models_update_priv _ _ _ _ t0 C $! hΣeq with "hΣt hΣ hΣΔ") => //.
+    - by iDestruct "Hle" as "[Hthis Hle]".
+    - by iApply expr_soundness.
   Qed.
 
   Lemma set_pub_soundness C Δ kd rigid Γ recv fld rhs fty exact_ t σ orig:
@@ -66,25 +73,41 @@ Section proofs.
     Forall wf_constraint Δ →
     expr_has_ty Δ Γ rigid kd recv (ClassT exact_ t σ) →
     has_field fld t Public fty orig →
-    expr_has_ty Δ Γ rigid kd rhs (subst_ty σ fty) →
+    (is_true exact_ ∨ no_this fty) →
+    expr_has_ty Δ Γ rigid kd rhs (subst_fty exact_ t σ fty) →
+    ∀ t0 t0def Σt0 σ0,
+    pdefs !! t0 = Some t0def →
+    length Σt0 = length t0def.(generics) →
+    inherits_using t0 C σ0 →
     ∀ Σ st st' n,
     length Σ = rigid →
     cmd_eval C st (SetC recv fld rhs) st' n →
+    let Σthis0 := interp_exact_tag interp_type t0 Σt0 in
+    ⌜interp_list interp_nothing Σt0 σ0 ≡ Σ⌝ -∗
+    □ interp_env_as_mixed Σt0 -∗
     □ interp_env_as_mixed Σ -∗
-    □ Σinterp Σ Δ -∗
-    heap_models st.2 ∗ interp_local_tys Σ Γ st.1 -∗
-    |=▷^n heap_models st'.2 ∗ interp_local_tys Σ Γ st'.1.
+    □ Σinterp Σthis0 Σ Δ -∗
+    heap_models st.2 ∗ interp_local_tys Σthis0 Σ Γ st.1 -∗
+    |=▷^n heap_models st'.2 ∗ interp_local_tys Σthis0 Σ Γ st'.1.
   Proof.
-    move => wfpdefs wflty ? hrecv hf hrhs Σ st st' n hrigid hc.
+    move => wfpdefs wflty ? hrecv hf hex hrhs.
+    move => t0 t0def Σt0 σ0 ht0def hlenΣt0 hin0.
+    move => Σ st st' n hrigid hc.
     elim/cmd_eval_setI : hc => {n}.
-    move => Ω h l v t0 vs vs' heval heval_rhs hheap -> hvis.
-    iIntros "#hΣ #hΣΔ".
+    move => Ω h vis fty0 orig0 l v t1 vs vs' heval heval_rhs hheap ->.
+    move => hf0 hvis Σthis0.
+    iIntros "%heqΣ #hΣt0 #hΣ #hΣΔ".
     iIntros "[Hh #Hle]" => /=.
     iSplitL; last done.
     assert (ht: wf_ty (ClassT exact_ t σ)) by (by apply expr_has_ty_wf in hrecv).
-    assert (htt: wf_ty (ClassT true t σ)).
-    { by eapply wf_ty_exact. }
-    iApply (heap_models_update _ _ _ _ _ _ exact_ t σ) => //=; try (by apply wfpdefs).
+    iAssert (□ interp_as_mixed Σthis0)%I as "#hΣthis".
+    { iModIntro; iIntros (w) "hw".
+      iLeft; iRight; iRight.
+      iExists t0, Σt0, t0def; iSplit; first done.
+      by iApply (exact_subtype_is_inclusion_aux with "hΣt0 hw").
+    }
+    iApply ((heap_models_update_pub _ _ _ _ _ _ exact_ t σ)
+      with "hΣt0 hΣ") => //=; try (by apply wfpdefs).
     - iApply expr_soundness => //; by apply wfpdefs.
     - iApply expr_soundness => //; by apply wfpdefs.
   Qed.
