theories/soundness/sub.v
@@ -15,52 +15,72 @@ From shack Require Import eval heap modality interp typing.
 From shack.soundness Require Import defs.
 
 Section proofs.
-  (* assume a given set of class definitions *)
-  Context `{PDC: ProgDefContext}.
-  (* assume some SDT constraints and their properties *)
-  Context `{SDTCS: SDTClassSpec}.
+  (* assume a given set of class definitions and their SDT annotations. *)
+  Context `{SDTCVS: SDTClassVarianceSpec}.
 
   (* Iris semantic context *)
   Context `{!sem_heapGS Θ}.
 
-  Lemma sub_soundness C Δ kd Γ rigid Γ0 Γ1 c:
+  Lemma sub_soundness C cdef Δ kd Γ rigid Γ0 Γ1 c:
     wf_cdefs pdefs →
     wf_lty Γ →
     bounded_lty rigid Γ →
-    ok_ty Δ (this_type Γ) →
     Forall wf_constraint Δ →
     Forall (bounded_constraint rigid) Δ →
+    pdefs !! C = Some cdef →
     lty_sub Δ kd Γ1 Γ0 →
     bounded_lty rigid Γ0 →
     cmd_has_ty C Δ kd rigid Γ c Γ1 →
+    ∀ t0 t0def Σt0 σ0,
+    pdefs !! t0 = Some t0def →
+    length Σt0 = length t0def.(generics) →
+    inherits_using t0 C σ0 →
     ∀ Σ st st' n,
     length Σ = rigid →
+    rigid ≥ length cdef.(generics) →
     cmd_eval C st c st' n →
+    let Σthis := interp_exact_tag interp_type t0 Σt0 in
+    ⌜interp_list interp_nothing Σt0 σ0 ≡ Σ⌝ -∗
+    □ interp_env_as_mixed Σt0 -∗
     □ interp_env_as_mixed Σ -∗
-    □ Σinterp Σ Δ -∗
-    □ (⌜wf_lty Γ⌝
-         → ⌜bounded_lty rigid Γ⌝
-           → ⌜ok_ty Δ (this_type Γ)⌝
-             → ⌜Forall wf_constraint Δ⌝
-               → ⌜Forall (bounded_constraint rigid) Δ⌝
-                 → ∀ (a : list (interp Θ)) (a0 a1 : local_env * heap)
-                     (a2 : nat),
-                     ⌜length a = rigid⌝ -∗
-                     ⌜cmd_eval C a0 c a1 a2⌝ -∗
-                     □ interp_env_as_mixed a -∗
-                     □ Σinterp a Δ -∗
-                     heap_models a0.2 ∗ interp_local_tys a Γ a0.1 -∗
-                     |=▷^a2 heap_models a1.2 ∗ interp_local_tys a Γ1 a1.1) -∗
-    heap_models st.2 ∗ interp_local_tys Σ Γ st.1 -∗
-    |=▷^n heap_models st'.2 ∗ interp_local_tys Σ Γ0 st'.1.
+    □ Σinterp Σthis Σ Δ -∗
+
+    □ (⌜wf_lty Γ⌝ →
+       ⌜bounded_lty rigid Γ⌝ →
+       ⌜Forall wf_constraint Δ⌝ →
+       ⌜Forall (bounded_constraint rigid) Δ⌝ →
+       ∀ Σ st st' n,
+       ⌜length Σ = rigid⌝ →
+       ⌜rigid ≥ length (generics cdef)⌝ →
+       ⌜ cmd_eval C st c st' n⌝ →
+       ⌜interp_list interp_nothing Σt0 σ0 ≡ Σ⌝ -∗
+       □ interp_env_as_mixed Σt0 -∗
+       □ interp_env_as_mixed Σ -∗
+       □ Σinterp (interp_exact_tag interp_type t0 Σt0) Σ Δ -∗
+       heap_models st.2 ∗
+         interp_local_tys (interp_exact_tag interp_type t0 Σt0) Σ Γ st.1 -∗
+       |=▷^n heap_models st'.2 ∗
+         interp_local_tys (interp_exact_tag interp_type t0 Σt0) Σ Γ1 st'.1) -∗
+
+    heap_models st.2 ∗ interp_local_tys Σthis Σ Γ st.1 -∗
+    |=▷^n heap_models st'.2 ∗ interp_local_tys Σthis Σ Γ0 st'.1.
   Proof.
-    move => wfpdefs wflty blty hokthis hΔ hΔb hsub hb h Σ st st' n hrigid hc.
-    iIntros "#hΣ #hΣΔ #HI".
-    iIntros "H".
-    iSpecialize ("HI" $! wflty blty hokthis hΔ hΔb _ _ _ _ hrigid with "[//] hΣ hΣΔ H").
+    move => wfpdefs wflty blty hΔ hΔb hcdef hsub hb h.
+    move => t0 t0def Σt0 σ0 ht0def hlenΣt0 hin_t0_C.
+    move => Σ st st' n hrigid hge hc Σthis.
+    iIntros "%hΣeq #hΣt0 #hΣ #hΣΔ #HI H".
+    iSpecialize ("HI" $! wflty blty hΔ hΔb).
+    iSpecialize ("HI" $! Σ _ _ _ hrigid hge hc hΣeq with "hΣt0 hΣ hΣΔ H").
     iApply updN_mono_I; last done.
-    iIntros "[Hh #Hrty]". iFrame.
-    iDestruct (interp_local_tys_is_inclusion with "hΣ hΣΔ Hrty") as "Hrty'" => //; try by apply wfpdefs.
+    iIntros "[Hh #Hrty]".
+    iFrame.
+    iAssert (□ interp_as_mixed Σthis)%I as "#hΣthis".
+    { iModIntro; iIntros (w) "hw".
+      iLeft; iRight; iRight.
+      iExists t0, Σt0, t0def; iSplit; first done.
+      by iApply (exact_subtype_is_inclusion_aux with "hΣt0 hw").
+    }
+    iDestruct (interp_local_tys_is_inclusion with "hΣthis hΣ hΣΔ Hrty") as "Hrty'" => //; try by apply wfpdefs.
     + apply cmd_has_ty_wf in h; try (assumption || by apply wfpdefs).
     + rewrite Forall_forall => i hi v.
       by apply _.
